cedar-lean/Cedar/Thm/Validation/Typechecker/GetAttr.lean
@@ -32,36 +32,43 @@ theorem getAttrInRecord_has_empty_capabilities {x₁ : Expr} {a : Attr} {c₁ c�
 := by
   intro h₁
   simp [getAttrInRecord] at h₁
-  split at h₁ <;> simp [ok, err] at h₁
-  simp [h₁]
-  split at h₁ <;> simp at h₁
+  split at h₁ <;>
+  (try split at h₁) <;>
+  simp [ok, err] at h₁ <;>
   simp [h₁]
 
-theorem type_of_getAttr_inversion {x₁ : Expr} {a : Attr} {c₁ c₂ : Capabilities} {env : Environment} {ty : CedarType}
+theorem type_of_getAttr_inversion {x₁ : Expr} {a : Attr} {c₁ c₂ : Capabilities} {env : Environment} {ty : TypedExpr}
   (h₁ : typeOf (Expr.getAttr x₁ a) c₁ env = Except.ok (ty, c₂)) :
   c₂ = ∅ ∧
   ∃ c₁',
-    (∃ ety, typeOf x₁ c₁ env = Except.ok (.entity ety, c₁')) ∨
-    (∃ rty, typeOf x₁ c₁ env = Except.ok (.record rty, c₁'))
+    (∃ ety, (typeOf x₁ c₁ env).typeOf = Except.ok (.entity ety, c₁')) ∨
+    (∃ rty, (typeOf x₁ c₁ env).typeOf = Except.ok (.record rty, c₁'))
 := by
   simp [typeOf] at h₁
   cases h₂ : typeOf x₁ c₁ env <;> simp [h₂] at h₁
   case ok res =>
     have ⟨ty₁, c₁'⟩ := res
-    simp [typeOfGetAttr] at h₁
+    simp [typeOfGetAttr, bind, Except.bind] at h₁
+    simp only [ResultType.typeOf, Except.map]
     split at h₁ <;> try contradiction
-    · simp only [List.empty_eq, Except.ok.injEq, Prod.mk.injEq, false_and, exists_const,
+    · simp [List.empty_eq, Except.ok.injEq, Prod.mk.injEq, false_and, exists_const,
         CedarType.record.injEq, exists_and_right, exists_eq', true_and, false_or, and_true, reduceCtorEq]
-      apply getAttrInRecord_has_empty_capabilities h₁
+      split at h₁ <;> simp [ok] at h₁
+      rename_i heq₁ _ _ heq₂
+      simp [heq₁, ←h₁]
+      apply getAttrInRecord_has_empty_capabilities heq₂
     · simp only [List.empty_eq, Except.ok.injEq, Prod.mk.injEq, CedarType.entity.injEq,
         exists_and_right, exists_eq', true_and, false_and, exists_const, or_false, and_true, reduceCtorEq]
       split at h₁ <;> try simp [err] at h₁
-      apply getAttrInRecord_has_empty_capabilities h₁
+      split at h₁ <;> simp [ok] at h₁
+      rename_i heq₁ _ _ _ _ _ heq₃
+      simp [heq₁, ←h₁]
+      apply getAttrInRecord_has_empty_capabilities heq₃
 
 theorem type_of_getAttr_is_sound_for_records {x₁ : Expr} {a : Attr} {c₁ c₁' : Capabilities} {env : Environment} {rty : RecordType} {request : Request} {entities : Entities} {v₁ : Value}
   (h₁ : CapabilitiesInvariant c₁ request entities)
   (h₂ : typeOf (Expr.getAttr x₁ a) c₁ env = Except.ok (ty, ∅))
-  (h₃ : typeOf x₁ c₁ env = Except.ok (CedarType.record rty, c₁'))
+  (h₃ : (typeOf x₁ c₁ env).typeOf = Except.ok (CedarType.record rty, c₁'))
   (h₄ : evaluate x₁ request entities = Except.ok v₁)
   (h₅ : InstanceOfType v₁ (CedarType.record rty)) :
   ∃ v,
@@ -69,41 +76,63 @@ theorem type_of_getAttr_is_sound_for_records {x₁ : Expr} {a : Attr} {c₁ c₁
    getAttr v₁ a entities = Except.error Error.extensionError ∨
    getAttr v₁ a entities = Except.error Error.arithBoundsError ∨
    getAttr v₁ a entities = Except.ok v) ∧
-   InstanceOfType v ty
+   InstanceOfType v ty.typeOf
 := by
   have ⟨r, h₆⟩ := instance_of_record_type_is_record h₅
   subst h₆
   simp [getAttr, attrsOf, Map.findOrErr]
-  simp only [typeOf, h₃, typeOfGetAttr, getAttrInRecord, List.empty_eq, Except.bind_ok] at h₂
+  split_type_of h₃ ; rename_i h₃ hl₃ hr₃
+  simp only [typeOf, hl₃, hr₃, typeOfGetAttr, getAttrInRecord, List.empty_eq, Except.bind_ok, bind, Except.bind] at h₂
   cases h₈ : Map.find? r a
   case none =>
     simp only [Except.error.injEq, reduceCtorEq, or_self, false_and, exists_const]
     split at h₂ <;> simp [ok, err] at h₂
+    rename_i heq
+    rw [h₃] at heq
+    simp at heq
+    subst heq
+    simp only [hl₃] at h₂
+    split at h₂ <;> simp at h₂
+    rename_i h₆
+    split at h₆ <;> try simp at h₆
     case h_1 _ _ h₉ =>
-      subst h₂
+      subst h₆
       have ⟨_, h₁₀⟩ := required_attribute_is_present h₅ h₉
       simp [h₈] at h₁₀
     case h_2 =>
-      split at h₂ <;> simp at h₂
-      subst h₂ ; rename_i h₁₀
+      split at h₆ <;> simp at h₆
+      subst h₆
+      rename_i h₁₀
       have ⟨_, h₁₁⟩ := capability_implies_record_attribute h₁ h₄ h₁₀
       simp [h₈] at h₁₁
   case some vₐ =>
     simp only [Except.ok.injEq, false_or, exists_eq_left', reduceCtorEq]
     split at h₂ <;> simp [ok, err] at h₂
+    rename_i h₆
+    rw [h₆] at h₃
+    simp at h₃
+    subst h₃
+    simp only [hl₃] at h₂
+    split at h₂ <;> simp at h₂
+    rename_i h₃
+    split at h₃ <;> try simp at h₃
     case h_1 _ _ h₉ =>
+      subst h₃
+      simp at h₂
       subst h₂
-      apply instance_of_attribute_type h₅ h₉ (by simp [Qualified.getType]) h₈
+      apply instance_of_attribute_type h₅ h₉ (by simp [Qualified.getType, TypedExpr.typeOf]) h₈
     case h_2 _ _ h₉ =>
-      split at h₂ <;> simp at h₂
+      split at h₃ <;> simp at h₃
+      subst h₃
+      simp at h₂
       subst h₂
-      apply instance_of_attribute_type h₅ h₉ (by simp [Qualified.getType]) h₈
+      apply instance_of_attribute_type h₅ h₉ (by simp [Qualified.getType, TypedExpr.typeOf]) h₈
 
 theorem type_of_getAttr_is_sound_for_entities {x₁ : Expr} {a : Attr} {c₁ c₁' : Capabilities} {env : Environment} {ety : EntityType} {request : Request} {entities : Entities} {v₁ : Value}
   (h₁ : CapabilitiesInvariant c₁ request entities)
   (h₂ : RequestAndEntitiesMatchEnvironment env request entities)
   (h₃ : typeOf (Expr.getAttr x₁ a) c₁ env = Except.ok (ty, ∅))
-  (h₄ : typeOf x₁ c₁ env = Except.ok (CedarType.entity ety, c₁'))
+  (h₄ : (typeOf x₁ c₁ env).typeOf = Except.ok (CedarType.entity ety, c₁'))
   (h₅ : evaluate x₁ request entities = Except.ok v₁)
   (h₆ : InstanceOfType v₁ (CedarType.entity ety)) :
   ∃ v,
@@ -111,68 +140,80 @@ theorem type_of_getAttr_is_sound_for_entities {x₁ : Expr} {a : Attr} {c₁ c�
    getAttr v₁ a entities = Except.error Error.extensionError ∨
    getAttr v₁ a entities = Except.error Error.arithBoundsError ∨
    getAttr v₁ a entities = Except.ok v) ∧
-   InstanceOfType v ty
+   InstanceOfType v ty.typeOf
 := by
   have ⟨uid, h₇, h₈⟩ := instance_of_entity_type_is_entity h₆
   subst h₈
   simp [getAttr, attrsOf, Entities.attrs, Map.findOrErr]
+  split_type_of h₄ ; rename_i h₄ hl₄ hr₄
   cases h₈ : Map.find? entities uid
   case none =>
     simp only [Except.bind_err, Except.error.injEq, or_self, or_false, true_and, reduceCtorEq]
-    exact type_is_inhabited ty
+    exact type_is_inhabited ty.typeOf
   case some d =>
     subst h₇
     simp only [Except.bind_ok]
     cases h₉ : Map.find? d.attrs a
     case none =>
       simp only [Except.error.injEq, or_self, false_and, exists_const]
-      simp only [typeOf, h₄, typeOfGetAttr, getAttrInRecord, List.empty_eq, Except.bind_ok] at h₃
+      simp only [typeOf, h₄, hl₄, typeOfGetAttr, getAttrInRecord, List.empty_eq, Except.bind_ok, bind, Except.bind] at h₃
       split at h₃ <;> simp [ok, err] at h₃
+      rename_i h₃₁
       split at h₃ <;> try simp at h₃
-      case h_1.h_1 _ _ h₁₀ _ _ h₁₁ =>
-        subst h₃
-        have h₁₂ := well_typed_entity_attributes h₂ h₈ h₁₀
+      rename_i h₃₂
+      split at h₃₂ <;> try simp at h₃₂
+      case h_1 _ _ _ _ _ h₁₁ =>
+        subst h₃₂
+        have h₁₂ := well_typed_entity_attributes h₂ h₈ h₃₁
         have ⟨aᵥ, h₁₃⟩ := required_attribute_is_present h₁₂ h₁₁
         simp [h₉] at h₁₃
-      case h_1.h_2 =>
-        split at h₃ <;> simp at h₃
-        subst h₃ ; rename_i h₁₃
+      case h_2 =>
+        split at h₃₂ <;> simp at h₃₂
+        subst h₃₂ ; rename_i h₁₃
         have ⟨_, h₁₄⟩ := capability_implies_entity_attribute h₁ h₅ h₈ h₁₃
         simp [h₉] at h₁₄
     case some vₐ =>
       simp only [Except.ok.injEq, false_or, exists_eq_left', reduceCtorEq]
-      simp [typeOf, h₄, typeOfGetAttr, getAttrInRecord] at h₃
+      simp [typeOf, h₄, hl₄, typeOfGetAttr, getAttrInRecord, bind, Except.bind] at h₃
       split at h₃ <;> simp [ok, err] at h₃
+      rename_i h₃₁
       split at h₃ <;> try simp at h₃
-      case h_1.h_1 _ _ h₁₀ _ _ h₁₁ =>
-        subst h₃
-        apply instance_of_attribute_type _ h₁₁ (by simp [Qualified.getType]) h₉
-        apply well_typed_entity_attributes h₂ h₈ h₁₀
-      case h_1.h_2 _ _ h₁₀ _ _ h₁₁ =>
-        split at h₃ <;> simp at h₃
-        subst h₃
-        apply instance_of_attribute_type _ h₁₁ (by simp [Qualified.getType]) h₉
-        apply well_typed_entity_attributes h₂ h₈ h₁₀
+      rename_i h₃₂
+      split at h₃₂ <;> try simp at h₃₂
+      case h_1 _ _ h₁₀ _ _ h₁₁ =>
+        subst h₃₂
+        cases h₃ ; subst ty
+        apply instance_of_attribute_type _ h₁₁ (by simp [Qualified.getType, TypedExpr.typeOf]) h₉
+        apply well_typed_entity_attributes h₂ h₈ h₃₁
+      case h_2 _ _ h₁₀ _ _ h₁₁ =>
+        split at h₃₂ <;> simp at h₃₂
+        subst h₃₂
+        cases h₃ ; subst ty
+        apply instance_of_attribute_type _ h₁₁ (by simp [Qualified.getType, TypedExpr.typeOf]) h₉
+        apply well_typed_entity_attributes h₂ h₈ h₃₁
 
-theorem type_of_getAttr_is_sound {x₁ : Expr} {a : Attr} {c₁ c₂ : Capabilities} {env : Environment} {ty : CedarType} {request : Request} {entities : Entities}
+theorem type_of_getAttr_is_sound {x₁ : Expr} {a : Attr} {c₁ c₂ : Capabilities} {env : Environment} {ty : TypedExpr} {request : Request} {entities : Entities}
   (h₁ : CapabilitiesInvariant c₁ request entities)
   (h₂ : RequestAndEntitiesMatchEnvironment env request entities)
   (h₃ : typeOf (Expr.getAttr x₁ a) c₁ env = Except.ok (ty, c₂))
   (ih : TypeOfIsSound x₁) :
   GuardedCapabilitiesInvariant (Expr.getAttr x₁ a) c₂ request entities ∧
-  ∃ v, EvaluatesTo (Expr.getAttr x₁ a) request entities v ∧ InstanceOfType v ty
+  ∃ v, EvaluatesTo (Expr.getAttr x₁ a) request entities v ∧ InstanceOfType v ty.typeOf
 := by
   have ⟨h₅, c₁', h₄⟩ := type_of_getAttr_inversion h₃
   subst h₅
   apply And.intro empty_guarded_capabilities_invariant
   rcases h₄ with ⟨ety, h₄⟩ | ⟨rty, h₄⟩ <;>
-  have ⟨_, v₁, h₆, h₇⟩ := ih h₁ h₂ h₄ <;>
+  split_type_of h₄ <;> rename_i h₄ hl₄ hr₄ <;>
+  have ⟨_, v₁, h₆, h₇⟩ := ih h₁ h₂ h₄  <;>
   simp [EvaluatesTo] at h₆ <;>
   simp [EvaluatesTo, evaluate] <;>
+  rw [hl₄] at h₇ <;>
   rcases h₆ with h₆ | h₆ | h₆ | h₆ <;> simp [h₆]
-  <;> try exact type_is_inhabited ty
-  · exact type_of_getAttr_is_sound_for_entities h₁ h₂ h₃ h₄ h₆ h₇
-  · exact type_of_getAttr_is_sound_for_records h₁ h₃ h₄ h₆ h₇
-
+  <;> try exact type_is_inhabited ty.typeOf
+  · have h₈ : (typeOf x₁ c₁ env).typeOf = Except.ok (CedarType.entity ety, c₁')  := by simp [h₄, hl₄, ResultType.typeOf, Except.map]; exact hr₄
+    exact type_of_getAttr_is_sound_for_entities h₁ h₂ h₃ h₈ h₆ h₇
+  · have h₈ : (typeOf x₁ c₁ env).typeOf = Except.ok (CedarType.record rty, c₁')  := by simp [h₄, hl₄, ResultType.typeOf, Except.map]; exact hr₄
+    exact type_of_getAttr_is_sound_for_records h₁ h₃ h₈ h₆ h₇
 
 end Cedar.Thm
