cedar-lean/Cedar/Thm/Validation/Typechecker/IfThenElse.lean
@@ -25,10 +25,10 @@ namespace Cedar.Thm
 open Cedar.Spec
 open Cedar.Validation
 
-theorem type_of_ite_inversion {x₁ x₂ x₃ : Expr} {c c' : Capabilities} {env : Environment} {ty : CedarType}
+theorem type_of_ite_inversion {x₁ x₂ x₃ : Expr} {c c' : Capabilities} {env : Environment} {ty : TypedExpr}
   (h₁ : typeOf (Expr.ite x₁ x₂ x₃) c env = Except.ok (ty, c')) :
   ∃ bty₁ c₁ ty₂ c₂ ty₃ c₃,
-    typeOf x₁ c env = .ok (.bool bty₁, c₁) ∧
+    (typeOf x₁ c env).typeOf = .ok (.bool bty₁, c₁) ∧
     match bty₁ with
     | .ff      =>
       typeOf x₃ c env = .ok (ty₃, c₃) ∧ ty = ty₃ ∧ c' = c₃
@@ -38,37 +38,41 @@ theorem type_of_ite_inversion {x₁ x₂ x₃ : Expr} {c c' : Capabilities} {env
     | .anyBool =>
       typeOf x₂ (c ∪ c₁) env = .ok (ty₂, c₂) ∧
       typeOf x₃ c env = .ok (ty₃, c₃) ∧
-      (ty₂ ⊔ ty₃) = (.some ty) ∧ c' = (c₁ ∪ c₂) ∩ c₃
+      (ty₂.typeOf ⊔ ty₃.typeOf) = (.some ty.typeOf) ∧ c' = (c₁ ∪ c₂) ∩ c₃
 := by
   simp [typeOf] at h₁
   cases h₂ : typeOf x₁ c env <;> simp [h₂, typeOfIf] at *
+  simp [ResultType.typeOf, Except.map]
   rename_i res₁
   split at h₁ <;> try { simp [ok, err] at h₁ } <;>
-  rename_i c₁ hr₁ <;> simp at hr₁ <;> have ⟨ht₁, hc₁⟩ := hr₁
+  rename_i c₁ hr₁
   case ok.h_1 =>
-    exists BoolType.tt, res₁.snd ; simp [←ht₁]
+    exists BoolType.tt, res₁.snd
+    simp [hr₁]
     cases h₃ : typeOf x₂ (c ∪ res₁.snd) env <;> simp [h₃] at h₁
     rename_i res₂ ; simp [ok] at h₁
     have ⟨ht₂, hc₂⟩ := h₁
     exists res₂.fst, res₂.snd
-    subst ht₂ hc₂ hc₁
-    simp only [and_self]
+    subst ht₂ hc₂
+    simp [h₃, ←hr₁]
   case ok.h_2 =>
-    exists BoolType.ff, res₁.snd ; simp [←ht₁]
+    exists BoolType.ff, res₁.snd
+    simp [hr₁]
     exact h₁
   case ok.h_3 =>
-    exists BoolType.anyBool, res₁.snd ; simp [←ht₁]
+    exists BoolType.anyBool, res₁.snd
+    simp [hr₁]
     cases h₃ : typeOf x₂ (c ∪ res₁.snd) env <;> simp [h₃] at h₁
     cases h₄ : typeOf x₃ c env <;> simp [h₄] at h₁
     split at h₁ <;> simp [ok, err] at h₁
-    rename_i ty' res₂ res₃ _ ty' hty
+    rename_i res₂ res₃ _ ty' h₅
     have ⟨ht, hc⟩ := h₁
-    subst ht hc hc₁
+    subst ht hc
     exists res₂.fst, res₂.snd
-    simp only [Except.ok.injEq, true_and]
+    simp only [←hr₁, h₃, Except.ok.injEq, true_and]
     exists res₃.fst, res₃.snd
 
-theorem type_of_ite_is_sound {x₁ x₂ x₃ : Expr} {c₁ c₂ : Capabilities} {env : Environment} {ty : CedarType} {request : Request} {entities : Entities}
+theorem type_of_ite_is_sound {x₁ x₂ x₃ : Expr} {c₁ c₂ : Capabilities} {env : Environment} {ty : TypedExpr} {request : Request} {entities : Entities}
   (h₁ : CapabilitiesInvariant c₁ request entities)
   (h₂ : RequestAndEntitiesMatchEnvironment env request entities)
   (h₃ : typeOf (Expr.ite x₁ x₂ x₃) c₁ env = Except.ok (ty, c₂))
@@ -76,11 +80,13 @@ theorem type_of_ite_is_sound {x₁ x₂ x₃ : Expr} {c₁ c₂ : Capabilities} 
   (ih₂ : TypeOfIsSound x₂)
   (ih₃ : TypeOfIsSound x₃) :
   GuardedCapabilitiesInvariant (Expr.ite x₁ x₂ x₃) c₂ request entities ∧
-  ∃ v, EvaluatesTo (Expr.ite x₁ x₂ x₃) request entities v ∧ InstanceOfType v ty
+  ∃ v, EvaluatesTo (Expr.ite x₁ x₂ x₃) request entities v ∧ InstanceOfType v ty.typeOf
 := by
   have ⟨bty₁, rc₁, ty₂, rc₂, ty₃, rc₃, h₄, h₅⟩ := type_of_ite_inversion h₃
+  split_type_of h₄ ; rename_i h₄ hl₄ hr₄
   specialize ih₁ h₁ h₂ h₄
   have ⟨ih₁₁, v₁, ih₁₂, ih₁₃⟩ := ih₁
+  simp [hl₄] at ih₁₃
   have ⟨b₁, hb₁⟩ := instance_of_bool_is_bool ih₁₃
   subst hb₁
   cases bty₁ <;> simp at h₅
@@ -90,11 +96,11 @@ theorem type_of_ite_is_sound {x₁ x₂ x₃ : Expr} {c₁ c₂ : Capabilities} 
     case false =>
       rcases ih₁₂ with ih₁₂ | ih₁₂ | ih₁₂ | ih₁₂ <;>
       simp [EvaluatesTo, evaluate, Result.as, ih₁₂, Coe.coe, Value.asBool, GuardedCapabilitiesInvariant] <;>
-      try exact type_is_inhabited ty
+      try exact type_is_inhabited ty.typeOf
       specialize ih₃ h₁ h₂ h₆
       have ⟨ih₃₁, v₃, ih₃₂, ih₃₃⟩ := ih₃
       rcases ih₃₂ with ih₃₂ | ih₃₂ | ih₃₂ | ih₃₂ <;> simp [ih₃₂] <;>
-      try exact type_is_inhabited ty
+      try exact type_is_inhabited ty.typeOf
       apply And.intro
       case left =>
         intro h₇ ; subst h₇ hc
@@ -107,9 +113,10 @@ theorem type_of_ite_is_sound {x₁ x₂ x₃ : Expr} {c₁ c₂ : Capabilities} 
     case true =>
       rcases ih₁₂ with ih₁₂ | ih₁₂ | ih₁₂ | ih₁₂ <;>
       simp [EvaluatesTo, evaluate, Result.as, ih₁₂, Coe.coe, Value.asBool, GuardedCapabilitiesInvariant] <;>
-      try exact type_is_inhabited ty
+      try exact type_is_inhabited ty.typeOf
       simp [GuardedCapabilitiesInvariant, ih₁₂] at ih₁₁
       have h₇ := capability_union_invariant h₁ ih₁₁
+      subst rc₁
       specialize ih₂ h₇ h₂ h₅
       have ⟨ih₂₁, v₂, ih₂₂, ih₂₃⟩ := ih₂
       apply And.intro
@@ -122,22 +129,23 @@ theorem type_of_ite_is_sound {x₁ x₂ x₃ : Expr} {c₁ c₂ : Capabilities} 
         exact capability_union_invariant ih₁₁ ih₂₁
       case right =>
         rcases ih₂₂ with ih₂₂ | ih₂₂ | ih₂₂ | ih₂₂ <;> simp [ih₂₂] <;>
-        try exact type_is_inhabited ty
+        try exact type_is_inhabited ty.typeOf
         apply instance_of_lub ht
         simp [ih₂₃]
   case tt =>
     have ⟨h₅, ht, hc⟩ := h₅
     rcases ih₁₂ with ih₁₂ | ih₁₂ | ih₁₂ | ih₁₂ <;>
     simp [EvaluatesTo, evaluate, Result.as, ih₁₂, Coe.coe, Value.asBool, GuardedCapabilitiesInvariant] <;>
-    try exact type_is_inhabited ty
+    try exact type_is_inhabited ty.typeOf
     have hb₁ := instance_of_tt_is_true ih₁₃
     simp at hb₁ ; subst hb₁ ; simp only [ite_true]
     simp [GuardedCapabilitiesInvariant, ih₁₂] at ih₁₁
     have h₆ := capability_union_invariant h₁ ih₁₁
+    subst rc₁
     specialize ih₂ h₆ h₂ h₅
     have ⟨ih₂₁, v₂, ih₂₂, ih₂₃⟩ := ih₂
     rcases ih₂₂ with ih₂₂ | ih₂₂ | ih₂₂ | ih₂₂ <;> simp [ih₂₂] <;>
-    try exact type_is_inhabited ty
+    try exact type_is_inhabited ty.typeOf
     subst ht hc ; simp [ih₂₃]
     intro h₇ ; subst h₇
     simp [GuardedCapabilitiesInvariant, ih₂₂] at ih₂₁
@@ -146,7 +154,7 @@ theorem type_of_ite_is_sound {x₁ x₂ x₃ : Expr} {c₁ c₂ : Capabilities} 
     have ⟨h₅, ht, hc⟩ := h₅
     rcases ih₁₂ with ih₁₂ | ih₁₂ | ih₁₂ | ih₁₂ <;>
     simp [EvaluatesTo, evaluate, Result.as, ih₁₂, Coe.coe, Value.asBool, GuardedCapabilitiesInvariant] <;>
-    try exact type_is_inhabited ty
+    try exact type_is_inhabited ty.typeOf
     have hb₁ := instance_of_ff_is_false ih₁₃
     simp at hb₁ ; simp [hb₁]
     specialize ih₃ h₁ h₂ h₅
