cedar-lean/Cedar/Thm/Validation/Typechecker/Or.lean
@@ -26,33 +26,31 @@ open Cedar.Data
 open Cedar.Spec
 open Cedar.Validation
 
-theorem type_of_or_inversion {x₁ x₂ : Expr} {c c' : Capabilities} {env : Environment} {ty : CedarType}
+theorem type_of_or_inversion {x₁ x₂ : Expr} {c c' : Capabilities} {env : Environment} {ty : TypedExpr}
   (h₁ : typeOf (Expr.or x₁ x₂) c env = Except.ok (ty, c')) :
   ∃ bty₁ c₁,
-    typeOf x₁ c env = .ok (.bool bty₁, c₁) ∧
+    (typeOf x₁ c env).typeOf = .ok (.bool bty₁, c₁) ∧
     if bty₁ = BoolType.tt
-    then ty = .bool BoolType.tt ∧ c' = ∅
+    then ty.typeOf = .bool BoolType.tt ∧ c' = ∅
     else ∃ bty₂ c₂,
-      typeOf x₂ c env = .ok (.bool bty₂, c₂) ∧
+      (typeOf x₂ c env).typeOf = .ok (.bool bty₂, c₂) ∧
       if bty₁ = BoolType.ff
-      then ty = .bool bty₂ ∧ c' = c₂
+      then ty.typeOf = .bool bty₂ ∧ c' = c₂
       else if bty₂ = BoolType.tt
-      then ty = .bool BoolType.tt ∧ c' = ∅
+      then ty.typeOf = .bool BoolType.tt ∧ c' = ∅
       else if bty₂ = BoolType.ff
-      then ty = .bool BoolType.anyBool ∧ c' = c₁
-      else ty = .bool BoolType.anyBool ∧ c' = c₁ ∩ c₂
+      then ty.typeOf = .bool BoolType.anyBool ∧ c' = c₁
+      else ty.typeOf = .bool BoolType.anyBool ∧ c' = c₁ ∩ c₂
 := by
   simp [typeOf] at h₁
   cases h₂ : typeOf x₁ c env <;> simp [h₂] at *
   rename_i res₁
   simp [typeOfOr] at h₁
   split at h₁ <;> simp [ok, err] at h₁ <;>
-  rename_i hr₁ <;> simp at hr₁ <;>
-  have ⟨ht₁, hc₁⟩ := hr₁
+  rename_i hr₁
   case ok.h_1 c₁  =>
-    exists BoolType.tt, c₁
-    have ⟨ht, hc⟩ := h₁
-    simp [←ht₁, ←hc₁, hc, ←ht]
+    exists BoolType.tt, res₁.snd
+    simp [←h₁, hr₁, ResultType.typeOf, Except.map]
   case ok.h_2 c₁ =>
     cases h₃ : typeOf x₂ c env <;> simp [h₃] at *
     rename_i res₂
@@ -60,47 +58,46 @@ theorem type_of_or_inversion {x₁ x₂ : Expr} {c c' : Capabilities} {env : Env
     rename_i bty₂ hr₂
     have ⟨ht, hc⟩ := h₁
     subst ht hc
-    exists BoolType.ff, c₁
-    simp [←ht₁, ←hc₁]
-    exists bty₂
-    simp [←hr₂]
-  case ok.h_3 bty₁ c₁ hneq₁ hneq₂ =>
+    exists BoolType.ff, res₁.snd
+    simp [hr₁, hr₂, ResultType.typeOf, Except.map]
+    simp [TypedExpr.typeOf]
+  case ok.h_3 bty₁ hneq₁ hneq₂ =>
     cases bty₁ <;> simp at hneq₁ hneq₂
-    exists BoolType.anyBool, c₁
-    simp [←ht₁, ←hc₁]
+    exists BoolType.anyBool, res₁.snd
+    simp [hr₁]
     cases h₃ : typeOf x₂ c env <;> simp [h₃] at *
     rename_i res₂
     split at h₁ <;> simp [ok, err] at h₁ <;>
     rename_i hr₂ <;>
-    have ⟨ht, hc⟩ := h₁ <;> subst ht hc <;> simp
+    have ⟨ht, hc⟩ := h₁ <;> subst ht hc <;> simp [hr₁, ResultType.typeOf, Except.map]
     case anyBool.ok.h_1 =>
       exists BoolType.tt, res₂.snd
-      simp [←hr₂]
     case anyBool.ok.h_2 =>
       exists BoolType.ff, res₂.snd
-      simp [←hr₂, ht₁, hc₁]
     case anyBool.ok.h_3 bty₂ hneq₁ hneq₂ =>
       exists bty₂, res₂.snd
-      simp [←hr₂, ←ht₁, ←hc₁]
+      simp [←hr₂, TypedExpr.typeOf]
       cases bty₂ <;> simp at *
 
-theorem type_of_or_is_sound {x₁ x₂ : Expr} {c₁ c₂ : Capabilities} {env : Environment} {ty : CedarType} {request : Request} {entities : Entities}
+theorem type_of_or_is_sound {x₁ x₂ : Expr} {c₁ c₂ : Capabilities} {env : Environment} {ty : TypedExpr} {request : Request} {entities : Entities}
   (h₁ : CapabilitiesInvariant c₁ request entities)
   (h₂ : RequestAndEntitiesMatchEnvironment env request entities)
   (h₃ : typeOf (Expr.or x₁ x₂) c₁ env = Except.ok (ty, c₂))
   (ih₁ : TypeOfIsSound x₁)
   (ih₂ : TypeOfIsSound x₂) :
   GuardedCapabilitiesInvariant (Expr.or x₁ x₂) c₂ request entities ∧
-  ∃ v, EvaluatesTo (Expr.or x₁ x₂) request entities v ∧ InstanceOfType v ty
+  ∃ v, EvaluatesTo (Expr.or x₁ x₂) request entities v ∧ InstanceOfType v ty.typeOf
 := by
   have ⟨bty₁, rc₁, h₄, h₅⟩ := type_of_or_inversion h₃
+  split_type_of h₄ ; rename_i h₄ hl₄ hr₄
   specialize ih₁ h₁ h₂ h₄
   have ⟨ih₁₁, v₁, ih₁₂, ih₁₃⟩ := ih₁
+  rw [hl₄] at ih₁₃
   have ⟨b₁, hb₁⟩ := instance_of_bool_is_bool ih₁₃ ; subst hb₁
   split at h₅
   case isTrue h₆ =>
     subst h₆
-    have ⟨hty, hc⟩ := h₅ ; subst hty hc
+    have ⟨hty, hc⟩ := h₅ ; rw [hty] at * ; subst hc
     apply And.intro empty_guarded_capabilities_invariant
     have h₇ := instance_of_tt_is_true ih₁₃
     simp at h₇ ; subst h₇
@@ -111,8 +108,10 @@ theorem type_of_or_is_sound {x₁ x₂ : Expr} {c₁ c₂ : Capabilities} {env :
     exact true_is_instance_of_tt
   case isFalse =>
     have ⟨bty₂, rc₂, h₅', h₇⟩ := h₅
+    split_type_of h₅' ; rename_i h₅' hl₅ hr₅
     specialize ih₂ h₁ h₂ h₅'
     have ⟨ih₂₁, v₂, ih₂₂, ih₂₃⟩ := ih₂
+    rw [hl₅] at ih₂₃
     have ⟨b₂, hb₂⟩ := instance_of_bool_is_bool ih₂₃
     subst hb₂
     simp [EvaluatesTo]
@@ -124,17 +123,17 @@ theorem type_of_or_is_sound {x₁ x₂ : Expr} {c₁ c₂ : Capabilities} {env :
     case false.inr.inr.inr.inr.inr.inr =>
       cases b₂ <;>
       simp [CoeT.coe, CoeHTCT.coe, CoeHTC.coe, CoeOTC.coe, CoeTC.coe, Coe.coe]
-      case false h₆ =>
+      case false h₆ _ _ =>
         cases bty₁ <;> simp at h₆ h₇
         case anyBool =>
           cases bty₂ <;> simp at h₇ <;>
-          have ⟨h₇, _⟩ := h₇ <;> subst h₇ <;>
+          have ⟨h₇, _⟩ := h₇ <;> rw [h₇] at * <;>
           try exact bool_is_instance_of_anyBool false
           exact ih₂₃
         case ff =>
           rw [h₇.left]
           exact ih₂₃
-      case true h₆ =>
+      case true h₆ _ _ =>
         cases bty₁ <;> cases bty₂ <;> simp at h₆ h₇ <;>
         have ⟨hty, hc⟩ := h₇ <;> simp [hty, hc] at *
         case ff.ff =>
@@ -151,10 +150,12 @@ theorem type_of_or_is_sound {x₁ x₂ : Expr} {c₁ c₂ : Capabilities} {env :
           apply And.intro
           · simp [GuardedCapabilitiesInvariant, ih₂₂] at ih₂₁
             apply capability_intersection_invariant
+            rw [←hr₅]
             simp [ih₂₁]
           · apply bool_is_instance_of_anyBool
         all_goals {
           simp [GuardedCapabilitiesInvariant, ih₂₂] at ih₂₁
+          rw [←hr₅]
           simp [ih₂₁]
           first
             | apply true_is_instance_of_tt
@@ -163,7 +164,7 @@ theorem type_of_or_is_sound {x₁ x₂ : Expr} {c₁ c₂ : Capabilities} {env :
     all_goals {
       simp [GuardedCapabilitiesInvariant] at ih₁₁ ih₂₁
       simp [ih₁₂] at ih₁₁ ; simp [ih₂₂] at ih₂₁
-      rename_i h₆
+      rename_i h₆ _ _
       rcases ih₁₃ with ⟨_, _, ih₁₃⟩
       simp [InstanceOfBoolType] at ih₁₃
       cases bty₁ <;> simp at h₆ ih₁₃ h₇
@@ -171,9 +172,10 @@ theorem type_of_or_is_sound {x₁ x₂ : Expr} {c₁ c₂ : Capabilities} {env :
       have ⟨ht, hc⟩ := h₇ <;> simp [ht, hc] at * <;>
       simp [true_is_instance_of_tt, bool_is_instance_of_anyBool] <;>
       try { apply empty_capabilities_invariant } <;>
+      subst rc₁ rc₂ <;>
       try { assumption }
       apply capability_intersection_invariant
-      simp [ih₁₁, ih₂₁]
+      simp [ih₁₁]
     }
 
 
