cedar-lean/Cedar/Thm/Validation/Typechecker/UnaryApp.lean
@@ -26,12 +26,12 @@ open Cedar.Data
 open Cedar.Spec
 open Cedar.Validation
 
-theorem type_of_not_inversion {x₁ : Expr} {c₁ c₂ : Capabilities} {env : Environment} {ty : CedarType}
+theorem type_of_not_inversion {x₁ : Expr} {c₁ c₂ : Capabilities} {env : Environment} {ty : TypedExpr}
   (h₁ : typeOf (Expr.unaryApp .not x₁) c₁ env = Except.ok (ty, c₂)) :
   c₂ = ∅ ∧
   ∃ bty c₁',
-    ty = .bool bty.not ∧
-    typeOf x₁ c₁ env = Except.ok (.bool bty, c₁')
+    ty.typeOf = .bool bty.not ∧
+    (typeOf x₁ c₁ env).typeOf = Except.ok (.bool bty, c₁')
 := by
   simp [typeOf] at h₁
   cases h₂ : typeOf x₁ c₁ env <;> simp [h₂] at h₁
@@ -39,25 +39,31 @@ theorem type_of_not_inversion {x₁ : Expr} {c₁ c₂ : Capabilities} {env : En
     have ⟨ty₁, c₁'⟩ := res
     simp [typeOfUnaryApp] at h₁
     split at h₁ <;> try contradiction
-    case h_1 _ ty₁ bty _ =>
+    case h_1 _ ty₁ bty _ h'₁ =>
       simp [ok] at h₁
       apply And.intro
       · simp [h₁]
       · exists bty, c₁'
-        simp only [and_true, h₁]
+        have ⟨ hl₁, _ ⟩ := h₁
+        rw [←hl₁]
+        simp only [TypedExpr.typeOf]
+        simp [ResultType.typeOf, Except.map, h'₁]
 
-theorem type_of_not_is_sound {x₁ : Expr} {c₁ c₂ : Capabilities} {env : Environment} {ty : CedarType} {request : Request} {entities : Entities}
+
+theorem type_of_not_is_sound {x₁ : Expr} {c₁ c₂ : Capabilities} {env : Environment} {ty : TypedExpr} {request : Request} {entities : Entities}
   (h₁ : CapabilitiesInvariant c₁ request entities)
   (h₂ : RequestAndEntitiesMatchEnvironment env request entities)
   (h₃ : typeOf (Expr.unaryApp .not x₁) c₁ env = Except.ok (ty, c₂))
   (ih : TypeOfIsSound x₁) :
   GuardedCapabilitiesInvariant (Expr.unaryApp .not x₁) c₂ request entities ∧
-  ∃ v, EvaluatesTo (Expr.unaryApp .not x₁) request entities v ∧ InstanceOfType v ty
+  ∃ v, EvaluatesTo (Expr.unaryApp .not x₁) request entities v ∧ InstanceOfType v ty.typeOf
 := by
   have ⟨h₅, bty, c₁', h₆, h₄⟩ := type_of_not_inversion h₃
-  subst h₅; subst h₆
+  subst h₅; rw [h₆]
+  split_type_of h₄ ; rename_i h₄ hl₄ hr₄
   apply And.intro empty_guarded_capabilities_invariant
   have ⟨_, v₁, h₆, h₇⟩ := ih h₁ h₂ h₄ -- IH
+  rw [hl₄] at h₇
   simp [EvaluatesTo] at h₆
   simp [EvaluatesTo, evaluate]
   rcases h₆ with h₆ | h₆ | h₆ | h₆ <;> simp [h₆]
@@ -83,11 +89,11 @@ theorem type_of_not_is_sound {x₁ : Expr} {c₁ c₂ : Capabilities} {env : Env
     exact type_is_inhabited (CedarType.bool (BoolType.not bty))
   }
 
-theorem type_of_neg_inversion {x₁ : Expr} {c₁ c₂ : Capabilities} {env : Environment} {ty : CedarType}
+theorem type_of_neg_inversion {x₁ : Expr} {c₁ c₂ : Capabilities} {env : Environment} {ty : TypedExpr}
   (h₁ : typeOf (Expr.unaryApp .neg x₁) c₁ env = Except.ok (ty, c₂)) :
   c₂ = ∅ ∧
-  ty = .int ∧
-  ∃ c₁', typeOf x₁ c₁ env = Except.ok (.int, c₁')
+  ty.typeOf = .int ∧
+  ∃ c₁', (typeOf x₁ c₁ env).typeOf = Except.ok (.int, c₁')
 := by
   simp [typeOf] at h₁
   cases h₂ : typeOf x₁ c₁ env <;> simp [h₂] at h₁
@@ -95,25 +101,29 @@ theorem type_of_neg_inversion {x₁ : Expr} {c₁ c₂ : Capabilities} {env : En
     have ⟨ty₁, c₁'⟩ := res
     simp [typeOfUnaryApp] at h₁
     split at h₁ <;> try contradiction
-    simp [ok] at h₁
-    simp [h₁]
+    rename_i h'₁
+    simp only [h'₁, ResultType.typeOf, Except.map, Except.ok.injEq, Prod.mk.injEq]
+    simp only [ok, Except.ok.injEq, Prod.mk.injEq] at h₁
+    simp [←h₁, TypedExpr.typeOf]
 
-theorem type_of_neg_is_sound {x₁ : Expr} {c₁ c₂ : Capabilities} {env : Environment} {ty : CedarType} {request : Request} {entities : Entities}
+theorem type_of_neg_is_sound {x₁ : Expr} {c₁ c₂ : Capabilities} {env : Environment} {ty : TypedExpr} {request : Request} {entities : Entities}
   (h₁ : CapabilitiesInvariant c₁ request entities)
   (h₂ : RequestAndEntitiesMatchEnvironment env request entities)
   (h₃ : typeOf (Expr.unaryApp .neg x₁) c₁ env = Except.ok (ty, c₂))
   (ih : TypeOfIsSound x₁) :
   GuardedCapabilitiesInvariant (Expr.unaryApp .neg x₁) c₂ request entities ∧
-  ∃ v, EvaluatesTo (Expr.unaryApp .neg x₁) request entities v ∧ InstanceOfType v ty
+  ∃ v, EvaluatesTo (Expr.unaryApp .neg x₁) request entities v ∧ InstanceOfType v ty.typeOf
 := by
   have ⟨h₅, h₆, c₁', h₄⟩ := type_of_neg_inversion h₃
-  subst h₅; subst h₆
+  subst h₅; rw [h₆]
   apply And.intro empty_guarded_capabilities_invariant
+  split_type_of h₄ ; rename_i h₄ hl₄ hr₄
   have ⟨_, v₁, h₆, h₇⟩ := ih h₁ h₂ h₄ -- IH
   simp [EvaluatesTo] at h₆
   simp [EvaluatesTo, evaluate]
   rcases h₆ with h₆ | h₆ | h₆ | h₆ <;> simp [h₆]
   case inr.inr.inr =>
+    rw [hl₄] at h₇
     have ⟨i, h₈⟩ := instance_of_int_is_int h₇
     subst h₈
     simp [apply₁, intOrErr]
@@ -128,11 +138,11 @@ theorem type_of_neg_is_sound {x₁ : Expr} {c₁ c₂ : Capabilities} {env : Env
     exact type_is_inhabited CedarType.int
   }
 
-theorem type_of_isEmpty_inversion {x₁ : Expr} {c₁ c₂ : Capabilities} {env : Environment} {ty : CedarType}
+theorem type_of_isEmpty_inversion {x₁ : Expr} {c₁ c₂ : Capabilities} {env : Environment} {ty : TypedExpr}
   (h₁ : typeOf (Expr.unaryApp .isEmpty x₁) c₁ env = Except.ok (ty, c₂)) :
   c₂ = ∅ ∧
-  ty = .bool .anyBool ∧
-  ∃ c₁' ty₀, typeOf x₁ c₁ env = Except.ok (.set ty₀, c₁')
+  ty.typeOf = .bool .anyBool ∧
+  ∃ c₁' ty₀, (typeOf x₁ c₁ env).typeOf = Except.ok (.set ty₀, c₁')
 := by
   simp [typeOf] at h₁
   cases h₂ : typeOf x₁ c₁ env <;> simp [h₂] at h₁
@@ -141,24 +151,28 @@ theorem type_of_isEmpty_inversion {x₁ : Expr} {c₁ c₂ : Capabilities} {env 
     simp [typeOfUnaryApp] at h₁
     split at h₁ <;> try contradiction
     simp [ok] at h₁
-    simp [h₁]
+    simp only [←h₁, List.empty_eq, TypedExpr.typeOf]
+    rename_i h₃
+    simp [h₃, ResultType.typeOf, Except.map]
 
-theorem type_of_isEmpty_is_sound {x₁ : Expr} {c₁ c₂ : Capabilities} {env : Environment} {ty : CedarType} {request : Request} {entities : Entities}
+theorem type_of_isEmpty_is_sound {x₁ : Expr} {c₁ c₂ : Capabilities} {env : Environment} {ty : TypedExpr} {request : Request} {entities : Entities}
   (h₁ : CapabilitiesInvariant c₁ request entities)
   (h₂ : RequestAndEntitiesMatchEnvironment env request entities)
   (h₃ : typeOf (Expr.unaryApp .isEmpty x₁) c₁ env = Except.ok (ty, c₂))
   (ih : TypeOfIsSound x₁) :
   GuardedCapabilitiesInvariant (Expr.unaryApp .isEmpty x₁) c₂ request entities ∧
-  ∃ v, EvaluatesTo (Expr.unaryApp .isEmpty x₁) request entities v ∧ InstanceOfType v ty
+  ∃ v, EvaluatesTo (Expr.unaryApp .isEmpty x₁) request entities v ∧ InstanceOfType v ty.typeOf
 := by
   have ⟨h₅, h₆, c₁', h₄⟩ := type_of_isEmpty_inversion h₃
-  subst h₅; subst h₆
+  subst h₅; rw [h₆]
   apply And.intro empty_guarded_capabilities_invariant
   replace ⟨ty₀, h₄⟩ := h₄
+  split_type_of h₄ ; rename_i h₄ hl₄ hr₄
   have ⟨_, v₁, h₆, h₇⟩ := ih h₁ h₂ h₄
   simp [EvaluatesTo, evaluate] at *
   rcases h₆ with h₆ | h₆ | h₆ | h₆ <;> simp [h₆]
   case inr.inr.inr =>
+    rw [hl₄] at h₇
     have ⟨s, h₈⟩ := instance_of_set_type_is_set h₇
     subst h₈
     simp [apply₁]
@@ -168,11 +182,11 @@ theorem type_of_isEmpty_is_sound {x₁ : Expr} {c₁ c₂ : Capabilities} {env :
     exact type_is_inhabited (.bool .anyBool)
   }
 
-theorem type_of_like_inversion {x₁ : Expr} {p : Pattern} {c₁ c₂ : Capabilities} {env : Environment} {ty : CedarType}
+theorem type_of_like_inversion {x₁ : Expr} {p : Pattern} {c₁ c₂ : Capabilities} {env : Environment} {ty : TypedExpr}
   (h₁ : typeOf (Expr.unaryApp (.like p) x₁) c₁ env = Except.ok (ty, c₂)) :
   c₂ = ∅ ∧
-  ty = .bool .anyBool ∧
-  ∃ c₁', typeOf x₁ c₁ env = Except.ok (.string, c₁')
+  ty.typeOf = .bool .anyBool ∧
+  ∃ c₁', (typeOf x₁ c₁ env).typeOf = Except.ok (.string, c₁')
 := by
   simp [typeOf] at h₁
   cases h₂ : typeOf x₁ c₁ env <;> simp [h₂] at h₁
@@ -181,24 +195,28 @@ theorem type_of_like_inversion {x₁ : Expr} {p : Pattern} {c₁ c₂ : Capabili
     simp [typeOfUnaryApp] at h₁
     split at h₁ <;> try contradiction
     simp [ok] at h₁
-    simp [h₁]
+    rename_i h'₁
+    simp only [ResultType.typeOf, Except.map, h'₁]
+    simp [←h₁, TypedExpr.typeOf]
 
-theorem type_of_like_is_sound {x₁ : Expr} {p : Pattern} {c₁ c₂ : Capabilities} {env : Environment} {ty : CedarType} {request : Request} {entities : Entities}
+theorem type_of_like_is_sound {x₁ : Expr} {p : Pattern} {c₁ c₂ : Capabilities} {env : Environment} {ty : TypedExpr} {request : Request} {entities : Entities}
   (h₁ : CapabilitiesInvariant c₁ request entities)
   (h₂ : RequestAndEntitiesMatchEnvironment env request entities)
   (h₃ : typeOf (Expr.unaryApp (.like p) x₁) c₁ env = Except.ok (ty, c₂))
   (ih : TypeOfIsSound x₁) :
   GuardedCapabilitiesInvariant (Expr.unaryApp (.like p) x₁) c₂ request entities ∧
-  ∃ v, EvaluatesTo (Expr.unaryApp (.like p) x₁) request entities v ∧ InstanceOfType v ty
+  ∃ v, EvaluatesTo (Expr.unaryApp (.like p) x₁) request entities v ∧ InstanceOfType v ty.typeOf
 := by
   have ⟨h₅, h₆, c₁', h₄⟩ := type_of_like_inversion h₃
-  subst h₅; subst h₆
+  subst h₅; rw [h₆]
   apply And.intro empty_guarded_capabilities_invariant
+  split_type_of h₄ ; rename_i h₄ hl₄ hr₄
   have ⟨_, v₁, h₆, h₇⟩ := ih h₁ h₂ h₄ -- IH
   simp [EvaluatesTo] at h₆
   simp [EvaluatesTo, evaluate]
   rcases h₆ with h₆ | h₆ | h₆ | h₆ <;> simp [h₆]
   case inr.inr.inr =>
+    rw [hl₄] at h₇
     have ⟨s, h₈⟩ := instance_of_string_is_string h₇
     subst h₈
     simp [apply₁]
@@ -207,12 +225,12 @@ theorem type_of_like_is_sound {x₁ : Expr} {p : Pattern} {c₁ c₂ : Capabilit
     exact type_is_inhabited (.bool .anyBool)
   }
 
-theorem type_of_is_inversion {x₁ : Expr} {ety : EntityType} {c₁ c₂ : Capabilities} {env : Environment} {ty : CedarType}
+theorem type_of_is_inversion {x₁ : Expr} {ety : EntityType} {c₁ c₂ : Capabilities} {env : Environment} {ty : TypedExpr}
   (h₁ : typeOf (Expr.unaryApp (.is ety) x₁) c₁ env = Except.ok (ty, c₂)) :
   c₂ = ∅ ∧
   ∃ ety' c₁',
-    ty = (.bool (if ety = ety' then .tt else .ff)) ∧
-    typeOf x₁ c₁ env = Except.ok (.entity ety', c₁')
+    ty.typeOf = (.bool (if ety = ety' then .tt else .ff)) ∧
+    (typeOf x₁ c₁ env).typeOf = Except.ok (.entity ety', c₁')
 := by
   simp [typeOf] at h₁
   cases h₂ : typeOf x₁ c₁ env <;> simp [h₂] at h₁
@@ -220,31 +238,34 @@ theorem type_of_is_inversion {x₁ : Expr} {ety : EntityType} {c₁ c₂ : Capab
     have ⟨ty₁, c₁'⟩ := res
     simp [typeOfUnaryApp] at h₁
     split at h₁ <;> try contradiction
-    case h_5 _ _ ety' h₃ =>
+    case h_5 _ _ ety' h₃ h'₁ =>
       simp only [UnaryOp.is.injEq] at h₃
-      subst h₃
+      rw [h₃] at h₁
       simp [ok] at h₁
       apply And.intro
       · simp [h₁]
       · exists ety', c₁'
-        simp only [h₁, and_self]
+        simp only [←h₁, h'₁, ResultType.typeOf, Except.map, and_true]
+        simp [TypedExpr.typeOf, h₃]
 
-theorem type_of_is_is_sound {x₁ : Expr} {ety : EntityType} {c₁ c₂ : Capabilities} {env : Environment} {ty : CedarType} {request : Request} {entities : Entities}
+theorem type_of_is_is_sound {x₁ : Expr} {ety : EntityType} {c₁ c₂ : Capabilities} {env : Environment} {ty : TypedExpr} {request : Request} {entities : Entities}
   (h₁ : CapabilitiesInvariant c₁ request entities)
   (h₂ : RequestAndEntitiesMatchEnvironment env request entities)
   (h₃ : typeOf (Expr.unaryApp (.is ety) x₁) c₁ env = Except.ok (ty, c₂))
   (ih : TypeOfIsSound x₁) :
   GuardedCapabilitiesInvariant (Expr.unaryApp (.is ety) x₁) c₂ request entities ∧
-  ∃ v, EvaluatesTo (Expr.unaryApp (.is ety) x₁) request entities v ∧ InstanceOfType v ty
+  ∃ v, EvaluatesTo (Expr.unaryApp (.is ety) x₁) request entities v ∧ InstanceOfType v ty.typeOf
 := by
   have ⟨h₅, ety', c₁', h₆, h₄⟩ := type_of_is_inversion h₃
-  subst h₅; subst h₆
+  subst h₅; rw [h₆]
   apply And.intro empty_guarded_capabilities_invariant
+  split_type_of h₄ ; rename_i h₄ hl₄ hr₄
   have ⟨_, v₁, h₆, h₇⟩ := ih h₁ h₂ h₄ -- IH
   simp [EvaluatesTo] at h₆
   simp [EvaluatesTo, evaluate]
   rcases h₆ with h₆ | h₆ | h₆ | h₆ <;> simp [h₆]
   case inr.inr.inr =>
+    rw [hl₄] at h₇
     have ⟨uid, h₈, h₉⟩ := instance_of_entity_type_is_entity h₇
     simp [apply₁, h₉, h₈]
     cases h₁₀ : ety == ety' <;>
@@ -256,13 +277,13 @@ theorem type_of_is_is_sound {x₁ : Expr} {ety : EntityType} {c₁ c₂ : Capabi
     apply type_is_inhabited
   }
 
-theorem type_of_unaryApp_is_sound {op₁ : UnaryOp} {x₁ : Expr} {c₁ c₂ : Capabilities} {env : Environment} {ty : CedarType} {request : Request} {entities : Entities}
+theorem type_of_unaryApp_is_sound {op₁ : UnaryOp} {x₁ : Expr} {c₁ c₂ : Capabilities} {env : Environment} {ty : TypedExpr} {request : Request} {entities : Entities}
   (h₁ : CapabilitiesInvariant c₁ request entities)
   (h₂ : RequestAndEntitiesMatchEnvironment env request entities)
   (h₃ : typeOf (Expr.unaryApp op₁ x₁) c₁ env = Except.ok (ty, c₂))
   (ih : TypeOfIsSound x₁) :
   GuardedCapabilitiesInvariant (Expr.unaryApp op₁ x₁) c₂ request entities ∧
-  ∃ v, EvaluatesTo (Expr.unaryApp op₁ x₁) request entities v ∧ InstanceOfType v ty
+  ∃ v, EvaluatesTo (Expr.unaryApp op₁ x₁) request entities v ∧ InstanceOfType v ty.typeOf
 := by
   match op₁ with
   | .not     => exact type_of_not_is_sound h₁ h₂ h₃ ih
