cedar-lean/Cedar/Validation/TypedExpr.lean
@@ -1,0 +1,156 @@
+/-
+ Copyright Cedar Contributors
+
+ Licensed under the Apache License, Version 2.0 (the "License");
+ you may not use this file except in compliance with the License.
+ You may obtain a copy of the License at
+
+      https://www.apache.org/licenses/LICENSE-2.0
+
+ Unless required by applicable law or agreed to in writing, software
+ distributed under the License is distributed on an "AS IS" BASIS,
+ WITHOUT WARRANTIES OR CONDITIONS OF ANY KIND, either express or implied.
+ See the License for the specific language governing permissions and
+ limitations under the License.
+-/
+
+import Cedar.Spec
+import Cedar.Validation.Types
+
+/-!
+This file defines a type annotated version of the Cedar AST
+-/
+
+namespace Cedar.Validation
+
+open Cedar.Data
+open Cedar.Spec
+
+/--
+A type annotated Cedar AST. This should have exactly the same variants as the
+unannotated `Expr` data type, but each variant carries an additional `ty` that
+stores the type of the expression.
+-/
+inductive TypedExpr where
+  | lit (p : Prim) (ty : CedarType)
+  | var (v : Var) (ty : CedarType)
+  | ite (cond : TypedExpr) (thenExpr : TypedExpr) (elseExpr : TypedExpr) (ty : CedarType)
+  | and (a : TypedExpr) (b : TypedExpr) (ty : CedarType)
+  | or (a : TypedExpr) (b : TypedExpr) (ty : CedarType)
+  | unaryApp (op : UnaryOp) (expr : TypedExpr) (ty : CedarType)
+  | binaryApp (op : BinaryOp) (a : TypedExpr) (b : TypedExpr) (ty : CedarType)
+  | getAttr (expr : TypedExpr) (attr : Attr) (ty : CedarType)
+  | hasAttr (expr : TypedExpr) (attr : Attr) (ty : CedarType)
+  | set (ls : List TypedExpr) (ty : CedarType)
+  | record (map : List (Attr × TypedExpr)) (ty : CedarType)
+  | call (xfn : ExtFun) (args : List TypedExpr) (ty : CedarType)
+
+
+deriving instance Repr, Inhabited for TypedExpr
+
+mutual
+
+def decTypedExpr (x y : TypedExpr) : Decidable (x = y) := by
+  cases x <;> cases y <;>
+  try { apply isFalse ; intro h ; injection h }
+  case lit.lit x₁ tx  y₁ ty  | var.var x₁ tx y₁ ty =>
+    exact match decEq x₁ y₁, decEq tx ty with
+    | isTrue h₁, isTrue h₂ => isTrue (by rw [h₁, h₂])
+    | isFalse _, _  | _, isFalse _ => isFalse (by intro h; injection h; contradiction)
+  case ite.ite x₁ x₂ x₃ tx y₁ y₂ y₃ ty =>
+    exact match decTypedExpr x₁ y₁, decTypedExpr x₂ y₂, decTypedExpr x₃ y₃, decEq tx ty with
+    | isTrue h₁, isTrue h₂, isTrue h₃, isTrue h₄ => isTrue (by rw [h₁, h₂, h₃, h₄])
+    | isFalse _, _, _, _ | _, isFalse _, _, _ | _, _, isFalse _, _ | _, _, _, isFalse _ => isFalse (by intro h; injection h; contradiction)
+  case and.and x₁ x₂ tx y₁ y₂ ty | or.or x₁ x₂ tx y₁ y₂ ty =>
+    exact match decTypedExpr x₁ y₁, decTypedExpr x₂ y₂, decEq tx ty with
+    | isTrue h₁, isTrue h₂, isTrue h₃ => isTrue (by rw [h₁, h₂, h₃])
+    | isFalse _, _, _ | _, isFalse _, _ | _, _, isFalse _ => isFalse (by intro h; injection h; contradiction)
+  case unaryApp.unaryApp o x₁ tx o' y₁ ty =>
+    exact match decEq o o', decTypedExpr x₁ y₁, decEq tx ty with
+    | isTrue h₁, isTrue h₂, isTrue h₃ => isTrue (by rw [h₁, h₂, h₃])
+    | isFalse _, _, _ | _, isFalse _, _ | _, _, isFalse _ => isFalse (by intro h; injection h; contradiction)
+  case binaryApp.binaryApp o x₁ x₂ tx o' y₁ y₂ ty =>
+    exact match decEq o o', decTypedExpr x₁ y₁, decTypedExpr x₂ y₂, decEq tx ty with
+    | isTrue h₁, isTrue h₂, isTrue h₃, isTrue h₄ => isTrue (by rw [h₁, h₂, h₃, h₄])
+    | isFalse _, _, _, _ | _, isFalse _, _, _ | _, _, isFalse _, _ | _, _, _, isFalse _ => isFalse (by intro h; injection h; contradiction)
+  case getAttr.getAttr x₁ a tx y₁ a' ty | hasAttr.hasAttr x₁ a tx y₁ a' ty =>
+    exact match decTypedExpr x₁ y₁, decEq a a', decEq tx ty with
+    | isTrue h₁, isTrue h₂, isTrue h₃ => isTrue (by rw [h₁, h₂, h₃])
+    | isFalse _, _, _ | _, isFalse _, _ | _, _, isFalse _ => isFalse (by intro h; injection h; contradiction)
+  case set.set xs tx ys ty =>
+    exact match decExprList xs ys, decEq tx ty with
+    | isTrue h₁, isTrue h₂ => isTrue (by rw [h₁, h₂])
+    | isFalse _, _ | _, isFalse _ => isFalse (by intro h; injection h; contradiction)
+  case record.record axs tx ays ty =>
+    exact match decProdAttrExprList axs ays, decEq tx ty with
+    | isTrue h₁, isTrue h₂ => isTrue (by rw [h₁, h₂])
+    | isFalse _, _ | _, isFalse _ => isFalse (by intro h; injection h; contradiction)
+  case call.call f xs tx f' ys ty =>
+    exact match decEq f f', decExprList xs ys, decEq tx ty with
+    | isTrue h₁, isTrue h₂, isTrue h₃ => isTrue (by rw [h₁, h₂, h₃])
+    | isFalse _, _, _ | _, isFalse _, _ | _, _, isFalse _ => isFalse (by intro h; injection h; contradiction)
+
+def decProdAttrExprList (axs ays : List (Prod Attr TypedExpr)) : Decidable (axs = ays) :=
+  match axs, ays with
+  | [], [] => isTrue rfl
+  | _::_, [] | [], _::_ => isFalse (by intro; contradiction)
+  | (a, x)::axs, (a', y)::ays =>
+    match decEq a a', decTypedExpr x y, decProdAttrExprList axs ays with
+    | isTrue h₁, isTrue h₂, isTrue h₃ => isTrue (by rw [h₁, h₂, h₃])
+    | isFalse _, _, _ | _, isFalse _, _ | _, _, isFalse _ =>
+      isFalse (by simp; intros; first | contradiction | assumption)
+
+def decExprList (xs ys : List TypedExpr) : Decidable (xs = ys) :=
+  match xs, ys with
+  | [], [] => isTrue rfl
+  | _::_, [] | [], _::_ => isFalse (by intro; contradiction)
+  | x::xs, y::ys =>
+    match decTypedExpr x y, decExprList xs ys with
+    | isTrue h₁, isTrue h₂ => isTrue (by rw [h₁, h₂])
+    | isFalse _, _ | _, isFalse _ => isFalse (by intro h; injection h; contradiction)
+end
+
+instance : DecidableEq TypedExpr := decTypedExpr
+
+def TypedExpr.typeOf : TypedExpr → CedarType
+  | lit _ ty
+  | var _ ty
+  | ite _ _ _ ty
+  | and _ _ ty
+  | or _ _ ty
+  | unaryApp _ _ ty
+  | binaryApp _ _ _ ty
+  | getAttr _ _ ty
+  | hasAttr _ _ ty
+  | set _ ty
+  | record _ ty
+  | call _ _ ty => ty
+
+def TypedExpr.toExpr : TypedExpr → Expr
+  | lit p _ => Expr.lit p
+  | var v _ => Expr.var v
+  | ite cond thenExpr elseExpr _ => Expr.ite cond.toExpr thenExpr.toExpr elseExpr.toExpr
+  | and a b _ => Expr.and a.toExpr b.toExpr
+  | or a b _ => Expr.or a.toExpr b.toExpr
+  | unaryApp op expr _ => Expr.unaryApp op expr.toExpr
+  | binaryApp op a b _ => Expr.binaryApp op a.toExpr b.toExpr
+  | getAttr expr attr _ => Expr.getAttr expr.toExpr attr
+  | hasAttr expr attr _ => Expr.hasAttr expr.toExpr attr
+  | set ls ty => Expr.set $ ls.map₁ (λ ⟨e, h₁⟩  =>
+    have _ : sizeOf e < 1 + sizeOf ls + sizeOf ty := by
+      have := List.sizeOf_lt_of_mem h₁
+      omega
+    e.toExpr)
+  | record ls ty => Expr.record $ ls.map₁ (λ ⟨(a, e), h₁⟩  =>
+    have _ : sizeOf e < 1 + sizeOf ls + sizeOf ty := by
+      have := Map.sizeOf_lt_of_value h₁
+      simp only [Map.mk.sizeOf_spec] at this
+      omega
+    (a, e.toExpr))
+  | call xfn args ty => Expr.call xfn $ args.map₁ (λ ⟨e, h₁⟩ =>
+    have _ : sizeOf e < 1 + sizeOf args + sizeOf ty := by
+      have := List.sizeOf_lt_of_mem h₁
+      omega
+    e.toExpr)
+
+end Cedar.Validation
